changes on add & next Waypoint & testing

Drone.dfy
@@ -28,7 +28,7 @@ class Drone {
         
         0 < r && 0 < n && 
         
-        verifyBoundaries(x,y,z)
+       verifyBoundaries(x,y,z)
         
         
     }
@@ -53,9 +53,8 @@ class Drone {
 
     
 
-    
 
-    function verifyBoundaries(posX:int, posY:int, posZ:int) : bool
+    function method verifyBoundaries(posX:int, posY:int, posZ:int) : bool
     reads this`r, this`n
     {
         //Semisphere
@@ -67,25 +66,25 @@ class Drone {
         ( (posX*posX) + (posY*posY) <= (r*r) && 0<=posZ<=n )
     }
 
-    function verifySemisphere(posX:int, posY:int, posZ:int) : bool
+    function method verifySemisphere(posX:int, posY:int, posZ:int) : bool
     reads this`r, this`n
     {
         (posX*posX)+(posY*posY)+((posZ-n)*(posZ-n))<=(r*r) && n <= posZ
     }
 
-    function verifyIdle() : bool
+    function method verifyIdle() : bool
     reads this`z, this`curSpeed
     {
         z != 0 && curSpeed == 0
     }
     
-    function verifyMoving():bool
+    function method verifyMoving():bool
     reads this`z, this`curSpeed, this`maxSpeed
     {
         curSpeed == maxSpeed
     }
 
-    function verifyLanded():bool
+    function method verifyLanded():bool
     reads this`z, this`curSpeed
     {
         z == 0 && curSpeed == 0
@@ -93,18 +92,22 @@ class Drone {
     
     
 
-    function verifyPatrolling():bool 
-    reads this`x, this`y, this`z, this`r, this`n, this`curSpeed, this`maxSpeed
+    function method verifyPatrolling():bool 
+    reads this`x, this`y, this`z, this`r, this`n, this`curSpeed, this`maxSpeed, this`points
     {
         curSpeed == (maxSpeed/2)
 
         &&
 
-        verifySemisphere(x,y,z)
+        |points| > 0
+    }
+
+    function method verifyPoint():bool
+    reads this`points
+    {
+        points !=[]
     }
     
-
-
     method move(toX:int, toY:int, toZ:int)
     modifies this`targetX, this`targetY, this`targetZ, this`curSpeed
     requires RepInv()
@@ -116,10 +119,12 @@ class Drone {
     ensures verifyMoving()
     ensures targetZ != 0
     {
-        curSpeed := maxSpeed;
+        
         targetX := toX;
         targetY := toY;
         targetZ := toZ;
+
+        curSpeed := maxSpeed;
     }
 
     method completeMove()
@@ -132,59 +137,15 @@ class Drone {
     ensures RepInv()
     ensures verifySemisphere(x,y,z)
     {
-        curSpeed := 0;
-
+       
         x := targetX;
         y := targetY;
         z := targetZ;
+
+         curSpeed := 0;
     }
 
-    method addWaypoint(toX:int, toY:int, toZ:int)
-    modifies this`points, this`curSpeed
-    requires RepInv()
-    requires verifySemisphere(toX, toY, toZ)
-    requires points==[] ==> verifyIdle()
-    requires points!=[] ==> verifyPatrolling()
-    ensures RepInv()
-    {
-        var tuple: (int, int, int) := (toX, toY, toZ);
-        points := points + [tuple];
-    }
-
-    method changeWaypoint()
-    modifies this`targetX, this`targetY, this`targetZ, this`points, this`curSpeed
-    requires points!=[]
-    requires verifySemisphere(points[0].0, points[0].1, points[0].2)
-    ensures verifySemisphere(targetX, targetY, targetZ)
-    {
-      
-        targetX := points[0].0;
-        targetY :=points[0].1;
-        targetZ :=points[0].2;
-        points := points[1..];
-
-        curSpeed := maxSpeed/2; 
-       
-    }
-
-    method CompleteAddWaypoint()
-    modifies this`x, this`y, this`z, this`curSpeed
-    requires RepInv()
-    requires verifyPatrolling()
-    requires verifySemisphere(targetX, targetY, targetZ)
-    ensures verifySemisphere(x, y, z)
-    ensures points==[] ==> verifyIdle()
-    ensures points!=[] ==> verifyPatrolling()
-    {
-         if(points==[]){
-            curSpeed:=0;
-        }
-        x:=targetX;
-        y:=targetY;
-        z:=targetZ;
-
-       
-    }
+    
 
     method takeOff()
     modifies this`curSpeed
@@ -226,11 +187,64 @@ class Drone {
     ensures verifyLanded()
     ensures RepInv()
     {
-
         z := 0;
+
         curSpeed := 0;
     }
 
+    method addWaypoint(toX:int, toY:int, toZ:int)
+    modifies this`x, this`y, this`z, this`points, this`curSpeed
+    requires RepInv()
+    requires verifySemisphere(toX, toY, toZ)
+    requires points==[] ==> verifyIdle()
+    requires points!=[] ==> verifyPatrolling()
+    ensures RepInv()
+    ensures points==[] ==> verifyIdle()
+    ensures verifyPatrolling()
     
+    {
+        var tuple: (int, int, int) := (toX, toY, toZ);
+        points := points + [tuple];
+
+        
+        curSpeed:= maxSpeed/2;
+        
+
+    }
+
+    
+
+    
+
+    method nextWaypoint()
+    modifies this`x, this`y, this`z, this`points, this`curSpeed
+    requires points!=[]
+    requires verifySemisphere(points[0].0, points[0].1, points[0].2)
+    ensures verifySemisphere(x, y, z)
+    {
+      
+        x := points[0].0;
+        y :=points[0].1;
+        z :=points[0].2;
+        points := points[1..];
+
+        if(points==[]){
+            curSpeed:=0;
+        }
+       
+    }
+
+    static method Main() {
+        var drone := new Drone(5,9);
+        if(drone.verifyLanded()){
+            drone.takeOff();
+        }
+        if(drone.verifySemisphere(5,8,3) && drone.verifyIdle() && !drone.verifyPoint()){
+            drone.addWaypoint(5,8,3);
+        }
+        if(drone.verifyPoint() && drone.verifySemisphere(drone.points[0].0, drone.points[0].1, drone.points[0].2)){
+            drone.nextWaypoint();
+        }
+    }
 
 }
